Support local and scoped rules
This requires a major refactor of the rule set handling. We now use
one `ScopedEnvExtension` per `RuleSet`, just like `simp`.

Aesop/Test/Persistence3.lean
@@ -9,8 +9,8 @@ import Aesop.Test.Persistence2
 
 namespace Aesop
 
-@[aesop 50% (rule_sets [persistence2])]
+@[aesop 50% (rule_sets [test_persistence2])]
 def test (b : Bool) : NatOrBool := by
-  aesop (rule_sets [persistence1])
+  aesop (rule_sets [test_persistence1])
 
 end Aesop
