Aesop/Frontend/Attribute.lean
@@ -4,8 +4,8 @@ Released under Apache 2.0 license as described in the file LICENSE.
 Authors: Jannis Limperg
 -/
 
+import Aesop.Frontend.Extension
 import Aesop.Frontend.RuleExpr
-import Aesop.RuleSet
 
 open Lean
 open Lean.Elab
@@ -44,105 +44,20 @@ def «elab» (stx : Syntax) : TermElabM AttrConfig :=
 end AttrConfig
 
 
-inductive AttributeEntry
-  | rule (rsName : RuleSetName) (r : RuleSetMember)
-  | ruleSet (rsName : RuleSetName)
-
-initialize extension :
-    PersistentEnvExtension AttributeEntry AttributeEntry Aesop.RuleSets ← do
-  let ext ← registerPersistentEnvExtension {
-    name := `aesop
-    mkInitial := return {}
-    addImportedFn := λ entriess => do
-      let mut result := {}
-      for entries in entriess do
-        for entry in entries do
-          match entry with
-          | .rule rsName r => result := result.addRule rsName r
-          | .ruleSet rsName => result := result.ensureRuleSet rsName
-      return result
-    addEntryFn := λ
-      | rss, .rule rsName r => rss.addRule rsName r
-      | rss, .ruleSet rsName => rss.ensureRuleSet rsName
-    exportEntriesFn := λ rss => Id.run do
-      let mut result := #[]
-      for (rsName, _) in rss.others do
-        result := result.push $ .ruleSet rsName
-      for (rsName, r) in rss.globalRules do
-        result := result.push $ .rule rsName r
-      return result
-  }
-  let impl : AttributeImpl := {
-    name := `aesop
-    descr := "Register a declaration as an Aesop rule."
-    applicationTime := .afterCompilation
-    add := λ decl stx attrKind => withRef stx do
-      match attrKind with
-      | AttributeKind.global => pure ()
-      | _ => throwError "local and scoped Aesop rules are not supported."
-      let config ← runTermElabMAsCoreM $ AttrConfig.elab stx
-      let rules ← runMetaMAsCoreM $
-        config.rules.concatMapM (·.buildAdditionalGlobalRules decl)
-      let mut rss := ext.getState (← getEnv)
-      for (rule, rsNames) in rules do
-        for rsName in rsNames do
-          if ! rss.containsRuleSet rsName then throwError
-            "no such rule set: '{rsName}'\n  (Use 'declare_aesop_rule_set' to declare rule sets.)"
-          if rss.containsRule rsName rule.name then throwError
-            "'{rule.name.name}' is already registered in rule set '{rsName}'."
-          rss := rss.addRuleCore rsName rule
-      setEnv $ ext.setState (← getEnv) rss
-    erase := λ decl => do
-      let rss := ext.getState (← getEnv)
-      let rss ←
-        rss.eraseRulesChecked
-          { ruleSetNames := #[] }
-          { ident := RuleIdent.const decl, builders := #[], phases := #[] }
-      setEnv $ ext.setState (← getEnv) rss
-  }
-  -- Despite the name, this also works for non-builtin attributes.
-  registerBuiltinAttribute impl
-  return ext
-
-variable [Monad m] [MonadEnv m]
-
-def getAttributeRuleSets : m Aesop.RuleSets :=
-  return extension.getState (← getEnv)
-
--- These rule sets are used when `aesop` is called without any options.
-def getDefaultRuleSets (includeGlobalSimpTheorems := true) :
-    CoreM Aesop.RuleSets := do
-  let mut rss ← getAttributeRuleSets
-  if includeGlobalSimpTheorems then
-    let defaultSimpTheorems ← Meta.getSimpTheorems
-    let defaultRs :=
-      { rss.default with
-        normSimpLemmas := defaultSimpTheorems.merge rss.default.normSimpLemmas }
-    rss := { rss with default := defaultRs }
-  return rss
-
-def getDefaultRuleSet (includeGlobalSimpTheorems := true) :
-    CoreM Aesop.RuleSet := do
-  let rss ←
-    getDefaultRuleSets (includeGlobalSimpTheorems := includeGlobalSimpTheorems)
-  return rss.makeMergedRuleSet defaultEnabledRuleSets
-
-def modifyAttributeRuleSets
-    (f : Aesop.RuleSets → m Aesop.RuleSets) : m Unit := do
-  let env ← getEnv
-  let rss ← f $ extension.getState env
-  setEnv $ extension.setState env rss
-
-def isRuleSetDeclared (rsName : RuleSetName) : m Bool := do
-  let rss ← getAttributeRuleSets
-  return rss.containsRuleSet rsName
-
-def declareRuleSet [MonadError m] (rsName : RuleSetName) : m Unit := do
-  if rsName.isReserved then throwError
-    "rule set name '{rsName}' is reserved"
-  let rss ← getAttributeRuleSets
-  if rss.containsRuleSet rsName then throwError
-    "rule set '{rsName}' already declared"
-  setEnv $ extension.setState (← getEnv) $ rss.addEmptyRuleSet rsName
+initialize registerBuiltinAttribute {
+  name := `aesop
+  descr := "Register a declaration as an Aesop rule."
+  applicationTime := .afterCompilation
+  add := λ decl stx attrKind => withRef stx do
+    let config ← runTermElabMAsCoreM $ AttrConfig.elab stx
+    let rules ← runMetaMAsCoreM $
+      config.rules.concatMapM (·.buildAdditionalGlobalRules decl)
+    for (rule, rsNames) in rules do
+      for rsName in rsNames do
+        addRule rsName rule attrKind
+  erase := λ decl =>
+    eraseRules RuleSetNameFilter.all (RuleNameFilter.ofIdent $ .const decl)
+      (check := true)
+}
 
 end Aesop.Frontend
