Aesop/Frontend/Extension.lean
@@ -1,0 +1,103 @@
+/-
+Copyright (c) 2023 Jannis Limperg. All rights reserved.
+Released under Apache 2.0 license as described in the file LICENSE.
+Authors: Jannis Limperg
+-/
+
+import Aesop.Frontend.Extension.Init
+
+open Lean
+
+namespace Aesop.Frontend
+
+def extensionDescr (rsName : RuleSetName) :
+    SimpleScopedEnvExtension.Descr RuleSetMember RuleSet where
+  name := rsName
+  addEntry rs r := rs.add r
+  initial := ∅
+
+def declareRuleSetUnchecked (rsName : RuleSetName) : IO Unit := do
+  let ext ← registerSimpleScopedEnvExtension $ extensionDescr rsName
+  aesopExtensionsMapRef.modify (·.insert rsName ext)
+
+def isRuleSetDeclared (rsName : RuleSetName) : IO Bool :=
+  return (← aesopExtensionsMapRef.get).contains rsName
+
+variable [Monad m] [MonadError m] [MonadLiftT IO m]
+  [MonadLiftT (ST IO.RealWorld) m] [MonadEnv m] [MonadResolveName m]
+
+def checkRuleSetNotDeclared (rsName : RuleSetName) : m Unit := do
+  if ← isRuleSetDeclared rsName then
+    throwError "rule set '{rsName}' already exists"
+
+def declareRuleSet (rsName : RuleSetName) : m Unit := do
+  checkRuleSetNotDeclared rsName
+  declareRuleSetUnchecked rsName
+
+initialize builtinRuleSetNames.forM declareRuleSetUnchecked
+
+def getRuleSetExtension (rsName : RuleSetName) : m RuleSetExtension := do
+  let (some ext) := (← aesopExtensionsMapRef.get).find? rsName
+    | throwError "no such rule set: '{rsName}'\n  (Use 'declare_aesop_rule_set' to declare rule sets.\n   Declared rule sets are not visible in the current file; they only become visible once you import the declaring file.)"
+  return ext
+
+def getRuleSet (rsName : RuleSetName) (includeGlobalSimpTheorems : Bool) :
+    CoreM RuleSet := do
+  let rs := (← getRuleSetExtension rsName).getState (← getEnv)
+  if includeGlobalSimpTheorems && rsName == defaultRuleSetName then
+    let normSimpLemmas := (← Meta.getSimpTheorems).merge rs.normSimpLemmas
+    return { rs with normSimpLemmas }
+  else
+    return rs
+
+def getRuleSets (rsNames : Array RuleSetName)
+    (includeGlobalSimpTheorems : Bool) : CoreM RuleSets :=
+  rsNames.foldlM (init := ∅) λ rss rsName => do
+    let rs ← getRuleSet rsName includeGlobalSimpTheorems
+    return rss.addRuleSet rsName rs
+
+def getDefaultRuleSets (includeGlobalSimpTheorems : Bool) : CoreM RuleSets :=
+  getRuleSets defaultEnabledRuleSetNames includeGlobalSimpTheorems
+
+def getDefaultRuleSet (includeGlobalSimpTheorems : Bool) : CoreM RuleSet :=
+  return (← getDefaultRuleSets includeGlobalSimpTheorems).getMergedRuleSet
+
+def getAllRuleSets (includeGlobalSimpTheorems : Bool) : CoreM RuleSets := do
+  (← aesopExtensionsMapRef.get).foldM (init := ∅) λ rss rsName _ =>
+    return rss.addRuleSet rsName (← getRuleSet rsName includeGlobalSimpTheorems)
+
+def addRuleUnchecked (rsName : RuleSetName) (r : RuleSetMember)
+    (kind : AttributeKind) : m Unit := do
+  let ext ← getRuleSetExtension rsName
+  ext.add r kind
+
+def addRule (rsName : RuleSetName) (r : RuleSetMember) (kind : AttributeKind) :
+    m Unit := do
+  let ext ← getRuleSetExtension rsName
+  let rs := ext.getState (← getEnv)
+  if rs.contains r.name then
+    throwError "Rule '{r.name.name}' is already registered in rule set '{rsName}'."
+  ext.add r kind
+
+def eraseRules (rsf : RuleSetNameFilter) (rf : RuleNameFilter) (check : Bool) :
+    m Unit := do
+  match rsf.matchedRuleSetNames with
+  | none =>
+    let anyErased ←
+      (← aesopExtensionsMapRef.get).foldM (init := false) λ b _ ext => go b ext
+    if check && ! anyErased then
+      throwError "'{rf.ident.name}' is not registered (with the given features) in any rule set."
+  | some rsNames =>
+    let anyErased ←
+      rsNames.foldlM (init := false) λ b rsName => do
+        go b (← getRuleSetExtension rsName)
+    if check && ! anyErased then
+      throwError "'{rf.ident.name}' is not registered (with the given features) in any of the rule sets {rsNames.map toString}."
+  where
+    go (anyErased : Bool) (ext : RuleSetExtension) : m Bool := do
+      let env ← getEnv
+      let (rs, rsErased) := ext.getState env |>.erase rf
+      setEnv $ ext.modifyState env λ _ => rs
+      return anyErased || rsErased
+
+end Aesop.Frontend
