Aesop/Frontend/Extension/Init.lean
@@ -1,0 +1,22 @@
+/-
+Copyright (c) 2023 Jannis Limperg. All rights reserved.
+Released under Apache 2.0 license as described in the file LICENSE.
+Authors: Jannis Limperg
+-/
+
+import Aesop.RuleSet
+
+open Lean
+
+namespace Aesop
+
+/--
+An environment extension containing an Aesop rule set. Each rule set has its
+own extension.
+-/
+abbrev RuleSetExtension := SimpleScopedEnvExtension RuleSetMember RuleSet
+
+initialize aesopExtensionsMapRef : IO.Ref (HashMap Name RuleSetExtension) ←
+  IO.mkRef ∅
+
+end Aesop
