Aesop/Test/Persistence0.lean
@@ -1,9 +1,9 @@
 /-
-Copyright (c) 2022 Jannis Limperg. All rights reserved.
+Copyright (c) 2023 Jannis Limperg. All rights reserved.
 Released under Apache 2.0 license as described in the file LICENSE.
 Authors: Jannis Limperg
 -/
 
 import Aesop.Main
 
-declare_aesop_rule_sets [test_persistence2]
+declare_aesop_rule_sets [test_persistence1]
