Aesop/Test/Persistence1.lean
@@ -4,18 +4,16 @@ Released under Apache 2.0 license as described in the file LICENSE.
 Authors: Jannis Limperg
 -/
 
-import Aesop.Main
+import Aesop.Test.Persistence0
 
 namespace Aesop
 
-declare_aesop_rule_sets [persistence1]
-
-@[aesop 50% constructors (rule_sets [persistence1])]
+@[aesop 50% constructors (rule_sets [test_persistence1])]
 inductive NatOrBool where
   | ofNat (n : Nat)
   | ofBool (b : Bool)
 
 example (b : Bool) : NatOrBool := by
-  aesop (rule_sets [persistence1])
+  aesop (rule_sets [test_persistence1])
 
 end Aesop
