Aesop/Test/RuleSets1.lean
@@ -1,0 +1,91 @@
+/-
+Copyright (c) 2022-2023 Jannis Limperg. All rights reserved.
+Released under Apache 2.0 license as described in the file LICENSE.
+Authors: Jannis Limperg
+-/
+
+import Aesop.Test.RuleSets0
+
+set_option aesop.check.all true
+
+@[aesop safe (rule_sets [test_A])]
+inductive A : Prop where
+| intro
+
+@[aesop safe (rule_sets [test_B])]
+inductive B : Prop where
+| intro
+
+@[aesop safe]
+inductive C : Prop where
+| intro
+
+inductive D : Prop where
+| intro
+
+example : A := by
+  fail_if_success aesop (options := { terminal := true })
+  aesop (rule_sets [test_A])
+
+example : B := by
+  aesop (rule_sets [test_A, test_B])
+
+example : C := by
+  fail_if_success aesop (rule_sets [-default]) (options := { terminal := true })
+  aesop
+
+attribute [aesop safe (rule_sets [test_C])] C
+
+-- Removing the attribute removes all rules associated with C from all rule
+-- sets.
+attribute [-aesop] C
+
+example : C := by
+  fail_if_success aesop (rule_sets [test_C]) (options := { terminal := true })
+  aesop (add safe C)
+
+@[aesop norm simp]
+theorem ad : D ↔ A :=
+  ⟨λ _ => A.intro, λ _ => D.intro⟩
+
+example : D := by
+  aesop (rule_sets [test_A])
+
+attribute [-aesop] ad
+
+example : D := by
+  fail_if_success aesop (rule_sets [test_A]) (options := { terminal := true })
+  aesop (add norm ad) (rule_sets [test_A])
+
+-- Rules can also be local.
+
+inductive E : Prop where
+  | intro
+
+section
+
+attribute [local aesop safe] E
+
+example : E := by
+  aesop
+
+end
+
+example : E := by
+  fail_if_success aesop (options := { terminal := true })
+  constructor
+
+-- Rules can also be scoped.
+
+namespace EScope
+
+attribute [scoped aesop safe] E
+
+example : E := by
+  aesop
+
+end EScope
+
+example : E := by
+  fail_if_success aesop (options := { terminal := true })
+  open EScope in aesop
